abbreviated rules

theories/Compositional_Structures/Basic_Modules/Borda_Module_Ref.thy
@@ -3,7 +3,7 @@ theory Borda_Module_Ref
            "Component_Types/Elimination_Module_Ref"
 begin
 
-fun borda_score_mon :: "'a::{default, heap, hashable} Evaluation_Function_Ref" where
+definition borda_score_mon :: "'a::{default, heap, hashable} Evaluation_Function_Ref" where
   "borda_score_mon x A p =
     sum_impl (prefer_count_monadic_imp p x) A"
 
@@ -20,50 +20,33 @@ lemma borda_score_correct:
   assumes 
     fina: "finite A"
     and profrel: "(pl, pr) \<in> profile_rel"
-  shows "borda_score_mon x A pl \<le> SPEC (\<lambda> sc. sc = (borda_score x A pr))"
-  unfolding borda_score_mon.simps borda_score.simps
-  by (refine_vcg fina sum_impl_correct prefer_count_monadic_imp_correct  profrel)
+  shows "\<forall> a \<in> A. borda_score_mon a A pl \<le> SPEC (\<lambda> sc. sc = (borda_score a A pr))"
+  unfolding borda_score_mon_def borda_score.simps
+  by (safe, refine_vcg fina sum_impl_correct prefer_count_monadic_imp_correct profrel)
  
 
 lemma borda_ref_correct:          
   shows "(uncurry borda_ref, uncurry (RETURN oo borda)) \<in> 
   [\<lambda> (A, _). finite A]\<^sub>f (\<langle>Id\<rangle>set_rel \<times>\<^sub>r profile_rel)
   \<rightarrow> \<langle>\<langle>Id\<rangle>set_rel \<times>\<^sub>r \<langle>Id\<rangle>set_rel \<times>\<^sub>r \<langle>Id\<rangle>set_rel\<rangle>nres_rel"
-  unfolding borda_ref_def
-proof (intro frefI nres_relI,  clarsimp simp add: set_rel_id prod_rel_id simp del: borda.simps,
-    unfold borda.simps comp_apply SPEC_eq_is_RETURN(2)[symmetric], rename_tac A pl pr,
-refine_vcg)
+proof (intro frefI nres_relI, clarsimp simp del: max_eliminator.simps, rename_tac A pl pr)
   fix A:: "'a set"
   fix pl :: "'a Profile_List"
   fix pr :: "'a Profile"
   assume prel: " (pl, pr) \<in> profile_rel"
   assume fina: "finite A"
-  note csc = compute_scores_correct[where efnref = borda_score_mon and efn= borda_score
-and A = A and pl = pl
-      and pr = pr]
-  from fina prel this borda_score_correct have 
-    precompborda: "pre_compute_scores borda_score_mon A pl
-  \<le> SPEC (\<lambda>map. map = pre_computed_map borda_score A pr)" by fastforce
-  note maxelim = max_eliminator_ref_correct[where efn = borda_score and A = A and pl = pl
-      and pr = pr]
-  from fina prel this have mid: "(\<And>x. x = pre_computed_map borda_score A pr \<Longrightarrow>
-          max_eliminator_ref x A pl \<le> SPEC (\<lambda>x. x = max_eliminator borda_score A pr))"
-    by blast
-   show "  pre_compute_scores borda_score_mon A pl
-       \<le> SPEC (\<lambda>scores. max_eliminator_ref scores A pl \<le> SPEC (\<lambda>x. x = max_eliminator borda_score A pr))"
-     using precompborda  mid
-       SPEC_cons_rule[where m = "pre_compute_scores borda_score_mon A pl" and
-\<Psi> = "(\<lambda>scores. max_eliminator_ref scores A pl \<le> SPEC (\<lambda>x. x = max_eliminator borda_score A pr))"
-  and \<Phi> = "(\<lambda> map. map = (pre_computed_map borda_score A pr))"]
-     by blast
-qed 
+  show "borda_ref A pl \<le> RETURN (max_eliminator borda_score A pr)"
+    apply (unfold borda_ref_def RETURN_SPEC_conv)
+    using borda_score_correct max_eliminator_ref_correct_pc fina prel
+    by metis
+qed
 
 
 sepref_definition borda_elim_sep is
   "uncurry borda_ref":: 
     "(alts_set_impl_assn id_assn)\<^sup>k *\<^sub>a (profile_impl_assn id_assn)\<^sup>k 
    \<rightarrow>\<^sub>a (result_impl_assn id_assn)"
-  unfolding borda_ref_def  max_eliminator_ref_def borda_score_mon.simps sum_impl_def
+  unfolding borda_ref_def  max_eliminator_ref_def borda_score_mon_def sum_impl_def
     less_eliminator_ref_def  elimination_module_ref_def[abs_def] eliminate_def[abs_def]
     pre_compute_scores_def[abs_def] scoremax_def[abs_def] 
   apply (rewrite in "FOREACH _ _ \<hole>" hm.fold_custom_empty)
@@ -84,8 +67,19 @@ declare borda_elim_sep.refine [sepref_fr_rules]
 
 term borda_elim_sep
 
-lemmas borda_elim_sep_correct [sepref_fr_rules]
-  = borda_elim_sep.refine[FCOMP borda_ref_correct]
+
+find_theorems name: hr_comp
+
+lemma  borda_elim_sep_correct [sepref_fr_rules]:
+  shows "(uncurry borda_elim_sep, uncurry (RETURN \<circ>\<circ> borda))
+    \<in> [\<lambda>(a, b).
+           finite
+            a]\<^sub>a (alts_set_impl_assn id_assn)\<^sup>k *\<^sub>a
+                 (list_assn
+                   (hr_comp (ballot_impl_assn id_assn)
+                     ballot_rel))\<^sup>k \<rightarrow> result_impl_assn id_assn"
+  using borda_elim_sep.refine[FCOMP borda_ref_correct]
+  set_rel_id hr_comp_Id2 by simp
 
 
 
