theories/Compositional_Structures/Basic_Modules/Plurality_Module_Ref.thy
@@ -8,61 +8,73 @@ begin
 definition plur_score_ref :: "'a::{default, heap, hashable} Evaluation_Function_Ref" where
   "plur_score_ref x A p = (wc_fold p x)"
 
+lemma plur_score_correct:
+  fixes A:: "'a::{default, heap, hashable} set"
+  fixes pl:: "'a Profile_List" and pr:: "'a Profile"
+  assumes 
+    fina: "finite A"
+    and prel: "(pl, pr) \<in> profile_rel"
+    and profp: "profile A pr"
+  shows "\<forall> a \<in> A. plur_score_ref a A pl \<le> SPEC (\<lambda> sc. sc = (plur_score a A pr))"
+  unfolding plur_score_ref_def plur_score.simps
+proof safe
+  fix a :: 'a
+  from prel profp have profl: "profile_l A pl" using profile_ref by auto 
+  show "wc_fold pl a \<le> SPEC (\<lambda>sc. sc = win_count pr a) "
+    by (refine_vcg fina prel profl wc_fold_correct)
+qed
+
+definition pre_compute_plur_scores :: "'a set \<Rightarrow> 'a Profile_List \<Rightarrow> ('a \<rightharpoonup> nat) nres" 
+  where "pre_compute_plur_scores A pl \<equiv> do {
+   zeromap:: 'a Scores_Map  <- init_map A;
+  nfoldli pl (\<lambda>_. True) 
+    (\<lambda>ballot map. 
+     RETURN (if (length ballot > 0) then do {
+      let top = ballot!0;
+      let scx = the (map top);
+        (map(top\<mapsto>(Suc scx)))}
+       else map)
+    ) (zeromap)}"
+
+lemma plurality_map_correct:
+  fixes A:: "'a::{default, heap, hashable} set"
+  fixes pl:: "'a Profile_List" and pr:: "'a Profile"
+  assumes 
+    fina: "finite A"
+    and prel: "(pl, pr) \<in> profile_rel"
+    and profp: "profile A pr"
+  shows "pre_compute_plur_scores A p \<le> pre_compute_scores plur_score_ref A p"
+  unfolding pre_compute_plur_scores_def pre_compute_scores_def
+  plur_score_ref_def wc_fold_def
+  using assms empty_map
+  oops
+
 definition plurality_ref :: "'a::{default, heap, hashable} Electoral_Module_Ref" where
   "plurality_ref A pl \<equiv> do {
    scores <- (pre_compute_scores plur_score_ref A pl);
    max_eliminator_ref scores A pl
 }"
 
-lemma plur_score_refine_weak:
-  fixes A :: "'a set"
-  shows "(uncurry plurality_ref, uncurry (RETURN oo plurality)) \<in> 
+lemma plurality_ref_refine:
+  shows "(uncurry plurality_ref, uncurry (RETURN oo plurality_mod)) \<in> 
   ([\<lambda> (A, pl). finite_profile A
             pl]\<^sub>f (\<langle>Id\<rangle>set_rel \<times>\<^sub>r profile_rel)
    \<rightarrow> \<langle>\<langle>Id\<rangle>set_rel \<times>\<^sub>r \<langle>Id\<rangle>set_rel \<times>\<^sub>r \<langle>Id\<rangle>set_rel\<rangle>nres_rel)"
-proof (intro frefI nres_relI, unfold comp_apply, clarsimp simp del: plurality.simps, 
-        rename_tac A pr pl)
+proof (intro frefI nres_relI,  clarsimp simp del:  plurality_mod.simps plur_score.simps,
+     unfold plurality_ref_def plurality_mod.simps
+     RETURN_SPEC_conv, rename_tac A pl pr)
+  note max_eliminator_ref_correct_pc[where A = A and efn_ref = plur_score_ref and
+       efn = plur_score]
   fix A :: "'a set"
-  fix pr pl
+  fix pr :: "'a Profile"
+  fix pl :: "'a Profile_List"
   assume fina: "finite A"
-  assume profrel: "(pl, pr) \<in> profile_on_A_rel A"
-  from profrel have profl: "profile_l A ppl" using profile_prop_list
-    by blast
-  from profrel have prel: "(ppl, ppr) \<in> profile_rel" 
-    using profile_type_ref by blast
-  from  profl prel alteq wc_fold_correct 
-  show "wc_fold ppl x' \<le> SPEC (\<lambda>c. (c, win_count ppr x) \<in> nat_rel)"
-    by fastforce
-qed
-
-
-context profile_complete
-begin
-
-theorem plurality_elim_correct:
-  shows "(plurality_monadic A pl, (SPEC (\<lambda> em. em = plurality_mod A pr))) 
-  \<in> \<langle>\<langle>Id\<rangle>set_rel \<times>\<^sub>r \<langle>Id\<rangle>set_rel \<times>\<^sub>r \<langle>Id\<rangle>set_rel\<rangle>nres_rel"
-proof (unfold plurality_monadic_def plurality_mod.simps)
-  from fina nempa have arel: "(A, A) \<in> \<langle>Id\<rangle>alt_set_rel" 
-    unfolding alt_set_rel_def using in_br_conv[symmetric]
-    by (simp add: brI)
-  from profrel have prel: " (pl, pr) \<in> profile_rel" using profile_type_ref by blast
-  have prec: "pre_compute_scores plur_score_mon A pl 
-          \<le> SPEC (\<lambda> map. map = pre_computed_map plur_score A pr)"
-  using plur_score_refine_weak[where A = A]
-      compute_scores_correct_weak_evalref[THEN nres_relD, THEN refine_IdD]
-  by fastforce 
-  from arel prel show "(pre_compute_scores plur_score_mon A pl \<bind> (\<lambda>scores. max_eliminator_ref scores A pl),
-     SPEC (\<lambda>em. em = max_eliminator plur_score A pr))
-    \<in> \<langle>\<langle>Id\<rangle>set_rel \<times>\<^sub>r \<langle>Id\<rangle>set_rel \<times>\<^sub>r \<langle>Id\<rangle>set_rel\<rangle>nres_rel"
-   using prec max_eliminator_ref_correct[THEN fun_relD] specify_left[where M = 
-        "\<Down> (\<langle>Id\<rangle>set_rel \<times>\<^sub>r \<langle>Id\<rangle>set_rel \<times>\<^sub>r \<langle>Id\<rangle>set_rel) 
-  (SPEC (\<lambda>res. res = max_eliminator plur_score A pr))"
-       and m = "pre_compute_scores plur_score_mon A pl"
-       and \<Phi> = "(\<lambda>map. map = pre_computed_map plur_score A pr)"
-       and f = "(\<lambda>scores. max_eliminator_ref scores A pl)"] 
-  nres_relI nres_relD
-   by blast 
+  assume prel: "(pl, pr) \<in> profile_rel"
+  assume profp: "profile A pr"
+  show " pre_compute_scores plur_score_ref A pl \<bind> (\<lambda>scores. max_eliminator_ref scores A pl)
+       \<le> SPEC (\<lambda>x. x = max_eliminator plur_score A pr)"
+    using max_eliminator_ref_correct_pc plur_score_correct fina prel profp
+    by metis   
 qed
    
 
@@ -73,18 +85,18 @@ sepref_definition plurality_elim_sepref is
    \<rightarrow>\<^sub>a ((hs.assn nat_assn) \<times>\<^sub>a (hs.assn nat_assn) \<times>\<^sub>a (hs.assn nat_assn))"
   unfolding plurality_ref_def  max_eliminator_ref_def plur_score_ref_def
     less_eliminator_ref_def  elimination_module_ref_def[abs_def] eliminate_def[abs_def]
-    pre_compute_scores_def[abs_def] scoremax_def[abs_def] wc_fold_def[abs_def] short_circuit_conv
+    pre_compute_scores_def[abs_def] scoremax_def[abs_def] wc_fold_def[abs_def] 
+    short_circuit_conv
   apply (rewrite in "FOREACH _ _ \<hole>" hm.fold_custom_empty)
   apply (rewrite in "FOREACH _ _ \<hole>" hs.fold_custom_empty)
   apply (rewrite in "FOREACH _ _ \<hole>" hs.fold_custom_empty)
+  apply (rewrite in "RETURN ({}, {}, \<hole>)" hs.fold_custom_empty) 
+  apply (rewrite in "RETURN ({}, \<hole>, _)" hs.fold_custom_empty) 
+  apply (rewrite in "RETURN ( \<hole>, _, _)" hs.fold_custom_empty) 
   apply (rewrite in "_ \<bind> (\<lambda>(rej, def). if def = {} then RETURN (\<hole>, _, rej) else RETURN ({}, rej, def))" hs.fold_custom_empty)
   apply (rewrite in "_ \<bind> (\<lambda>(rej, def). if def = {} then RETURN (_, \<hole>, rej) else RETURN ({}, rej, def))" hs.fold_custom_empty)
   apply (rewrite in "_ \<bind> (\<lambda>(rej, def). if def = {} then RETURN (_, _, rej) else RETURN (\<hole>, rej, def))" hs.fold_custom_empty)
-
   apply sepref_dbg_keep
   done
 
-
-
-end
 end
