theories/Borda_Rule_Ref.thy
@@ -15,17 +15,25 @@ interpretation borda_rule_impl: elector_sepref borda_ref borda_elim_sep borda
   subgoal apply (intro frefI) using borda_ref_correct[THEN frefD] by auto
   done
 
+thm "borda_rule_impl.elector_sep_correct"
+
 lemma  borda_rule_correct [sepref_fr_rules]:
   shows "(uncurry borda_rule_sep, uncurry (RETURN oo borda_rule))
     \<in> [\<lambda>(A, pl).
            finite_profile A
             pl]\<^sub>a (hr_comp (hs.assn id_assn) (\<langle>Id\<rangle>set_rel))\<^sup>k *\<^sub>a
                   (list_assn
-                    (hr_comp (ballot_impl_assn id_assn)
-                      ballot_rel))\<^sup>k \<rightarrow> hr_comp (hs.assn id_assn) (\<langle>Id\<rangle>set_rel) \<times>\<^sub>a
+                    (hr_comp (arl_assn id_assn)
+                      (br (pl_\<alpha>) (distinct))))\<^sup>k
+
+                                     \<rightarrow> (hr_comp (hs.assn id_assn) (\<langle>Id\<rangle>set_rel) \<times>\<^sub>a
                                         hr_comp (hs.assn id_assn) (\<langle>Id\<rangle>set_rel) \<times>\<^sub>a
-                                        hr_comp (hs.assn id_assn) (\<langle>Id\<rangle>set_rel)"
-  unfolding borda_rule_sep_def borda_rule.simps using borda_rule_impl.elector_sep_correct .
+                                        hr_comp (hs.assn id_assn) (\<langle>Id\<rangle>set_rel))"
+ 
+  unfolding borda_rule_sep_def borda_rule.simps 
+  using borda_rule_impl.elector_sep_correct unfolding in_br_conv well_formed_pl_def
+  .
+  
 
 
 export_code borda_rule_sep in Scala_imp
